Turn CertiGC into a VSU

CertiGC/GC_Source/boxing.c
@@ -1,0 +1,26 @@
+#include "boxing.h"
+
+/* The following 5 functions should (in practice) compile correctly in CompCert,
+   but the CompCert correctness specification does not _require_ that
+   they compile correctly:  their semantics is "undefined behavior" in
+   CompCert C (and in C11), but in practice they will work in any compiler. */
+
+int test_int_or_ptr (value x) /* returns 1 if int, 0 if aligned ptr */ {
+    return (int)(((intnat)x)&1);
+}
+
+intnat int_or_ptr_to_int (value x) /* precondition: is int */ {
+    return (intnat)x;
+}
+
+void * int_or_ptr_to_ptr (value x) /* precond: is aligned ptr */ {
+    return (void *)x;
+}
+
+value int_to_int_or_ptr(intnat x) /* precondition: is odd */ {
+    return (value)x;
+}
+
+value ptr_to_int_or_ptr(void *x) /* precondition: is aligned */ {
+    return (value)x;
+}
