CertiGC/spec_boxing.v
@@ -1,0 +1,82 @@
+Require Import VST.floyd.proofauto.
+Require Import CertiGraph.CertiGC.boxing.
+#[export] Instance CompSpecs : compspecs. make_compspecs prog. Defined.
+Definition Vprog : varspecs. mk_varspecs prog. Defined.
+
+Local Open Scope logic.
+
+Definition valid_int_or_ptr (x: val) :=
+  match x with
+  | Vint i => if Archi.ptr64 then False else Int.testbit i 0 = true
+  | Vptr _ z => Ptrofs.testbit z 0 = false /\ Ptrofs.testbit z 1 = false
+  | Vlong i => if Archi.ptr64 then Int64.testbit i 0 = true else False
+  | _ => False
+  end.
+
+Definition test_int_or_ptr_spec :=
+ DECLARE _test_int_or_ptr
+ WITH x : val
+ PRE [int_or_ptr_type]
+   PROP (valid_int_or_ptr x)
+   PARAMS (x)
+   GLOBALS ()
+   SEP ()
+ POST [ tint ]
+   PROP()
+   RETURN(Vint (Int.repr (match x with
+                           | Vint _ => if Archi.ptr64 then 0 else 1
+                           | Vlong _ => if Archi.ptr64 then 1 else 0
+                           | _ => 0
+                           end)))
+   SEP().
+
+Definition int_or_ptr_to_int_spec :=
+  DECLARE _int_or_ptr_to_int
+  WITH x : val
+  PRE [int_or_ptr_type ]
+    PROP (is_int I32 Signed x)
+    PARAMS (x)
+    GLOBALS ()
+    SEP ()
+  POST [ (if Archi.ptr64 then tlong else tint) ]
+    PROP() RETURN (x) SEP().
+
+Definition int_or_ptr_to_ptr_spec :=
+  DECLARE _int_or_ptr_to_ptr
+  WITH x : val
+  PRE [int_or_ptr_type ]
+    PROP (isptr x)
+    PARAMS (x)
+    GLOBALS ()
+    SEP ()
+  POST [ tptr tvoid ]
+    PROP() RETURN (x) SEP().
+
+Definition int_to_int_or_ptr_spec :=
+  DECLARE _int_to_int_or_ptr
+  WITH x : val
+  PRE [ (if Archi.ptr64 then tlong else tint) ]
+    PROP (valid_int_or_ptr x)
+    PARAMS (x)
+    GLOBALS ()
+    SEP ()
+  POST [ int_or_ptr_type ]
+    PROP() RETURN (x) SEP().
+
+Definition ptr_to_int_or_ptr_spec :=
+  DECLARE _ptr_to_int_or_ptr
+  WITH x : val
+  PRE [tptr tvoid ]
+    PROP (valid_int_or_ptr x)
+    PARAMS (x)
+    GLOBALS ()
+    SEP()
+  POST [ int_or_ptr_type ]
+    PROP() RETURN (x) SEP().
+
+Definition Gprog: funspecs :=
+                     [test_int_or_ptr_spec;
+                      int_or_ptr_to_int_spec;
+                      int_or_ptr_to_ptr_spec;
+                      int_to_int_or_ptr_spec;
+                      ptr_to_int_or_ptr_spec].
