CertiGC/verif_boxing.v
@@ -1,0 +1,49 @@
+From VST Require Import floyd.proofauto floyd.VSU.
+From CertiGraph.CertiGC Require Import spec_boxing boxing.
+Local Open Scope logic.
+
+Axiom body_test_int_or_ptr: semax_body Vprog Gprog f_test_int_or_ptr test_int_or_ptr_spec.
+
+Lemma body_int_to_int_or_ptr:
+  semax_body Vprog Gprog f_int_to_int_or_ptr int_to_int_or_ptr_spec.
+Proof.
+  start_function.
+  forward.
+Qed.
+
+Lemma body_int_or_ptr_to_int:
+  semax_body Vprog Gprog f_int_or_ptr_to_int int_or_ptr_to_int_spec.
+Proof.
+  start_function.
+  red in H. destruct x; try easy.
+  forward.
+Qed.
+
+Lemma body_ptr_to_int_or_ptr:
+  semax_body Vprog Gprog f_ptr_to_int_or_ptr ptr_to_int_or_ptr_spec.
+Proof.
+  start_function.
+  forward.
+Qed.
+
+Lemma body_int_or_ptr_to_ptr:
+  semax_body Vprog Gprog f_int_or_ptr_to_ptr int_or_ptr_to_ptr_spec.
+Proof.
+  start_function.
+  forward.
+Qed.
+
+Definition Boxing_internal_specs: funspecs := Gprog.
+Definition Boxing_imported_specs:funspecs :=  nil.
+Definition Boxing_E : funspecs := nil.
+
+Definition BoxingVSU: @VSU NullExtension.Espec
+         Boxing_E Boxing_imported_specs ltac:(QPprog prog) Gprog (fun _ => emp).
+  Proof.
+    mkVSU prog Boxing_internal_specs.
+    - solve_SF_internal body_test_int_or_ptr.
+    - solve_SF_internal body_int_or_ptr_to_int.
+    - solve_SF_internal body_int_or_ptr_to_ptr.
+    - solve_SF_internal body_int_to_int_or_ptr.
+    - solve_SF_internal body_ptr_to_int_or_ptr.
+Qed.
