CertiGC/verif_gc.v
@@ -1,0 +1,119 @@
+Require Import VST.floyd.proofauto VST.floyd.VSU.
+From CertiGraph.CertiGC Require Import 
+   env_graph_gc
+   spec_gc verif_Is_from verif_create_heap verif_create_space
+   verif_do_generation verif_do_scan verif_forward verif_forward_roots
+   verif_garbage_collect verif_is_ptr verif_make_tinfo verif_resume.
+
+Local Open Scope logic.
+
+Definition GC_imported_specs:funspecs := 
+  MallocASI ++
+  [spec_boxing.test_int_or_ptr_spec; spec_boxing.int_or_ptr_to_ptr_spec;
+   spec_boxing.ptr_to_int_or_ptr_spec].
+
+(*    spec_malloc.MallocASI ++ 
+  [spec_boxing.test_int_or_ptr_spec; 
+   (*spec_boxing.int_or_ptr_to_int_spec; *)
+     spec_boxing.int_or_ptr_to_ptr_spec;
+    (* spec_boxing.int_to_int_or_ptr_spec;*)
+   spec_boxing.ptr_to_int_or_ptr_spec].
+*)
+
+Definition GC_E : funspecs := nil.
+
+Require Import String.
+
+Definition GCVSU: @VSU NullExtension.Espec
+         GC_E GC_imported_specs ltac:(QPprog gc_stack.prog) 
+         spec_gc.GC_ASI (all_string_constants Ews).
+  Proof.
+    mkVSU prog GC_Internal.
+intros.
+unfold Maps.PTree.prev in *; simpl in H.
+admit. (* need to take provide vacuous funspecs for,
+    garbage_collect_all certicoq_modify export_heap print_heapsize
+   reset_heap free_heap *)
+    - solve_SF_internal body_is_ptr.
+    - admit.  (* Is_from *)
+    - admit. (* abort *)
+    - solve_SF_internal body_forward.
+    - solve_SF_internal body_forward_roots.
+    - admit. (* forward_remset *)
+    - solve_SF_internal body_do_scan.
+    - solve_SF_internal body_do_generation.
+    - solve_SF_internal body_create_space.
+    - solve_SF_internal body_create_heap.
+    - solve_SF_internal body_make_tinfo.
+    - solve_SF_internal body_resume. 
+    - solve_SF_internal body_garbage_collect.
+    - admit. (* match up the string constants *)
+all: fail.
+Admitted.
+(*
+intros. unfold Vardefs; simpl.
+unfold all_string_constants; simpl.
+unfold InitGPred; simpl.
+Intros.
+
+
+Search cstring.
+repeat
+match goal with |- context [globvar2pred ?gv (?i, ?v)] =>
+  let i' := eval hnf in i in
+  let v' := eval hnf in v in
+  let x := constr:(init_data_list2pred gv (gvar_init v') (readonly2share (gvar_readonly v')) (gv i')) in
+  let x' := eval cbv [gvar_init gvar_readonly readonly2share 
+                      init_data_list2pred init_data2pred init_data_size] in x in
+  change (globvar2pred gv (i,v)) with x'
+end.
+Print Ltac do_string2bytes.
+
+repeat change (Int.zero_ext 8 ?x) with x.
+simpl Int.zero_ext.
+simpl init_data_list2pred.
+
+   (init_data_list2pred gv (gvar_init v') (readonly2share (gvar_readonly v')) (gv i'));
+  
+end.
+unfold gvar_init, gvar_readonly, readonly2share.
+
+cbv [globvar2pred].
+repeat change (gvar_volatile _) with false.
+cbv match.
+
+simpl gvar_init.
+match goal with |- context [globvar2pred ?gv (?i, ?v)] =>
+
+change (globvar2pred _ (_, v___stderrp)) with emp.
+rewrite !sepcon_assoc.
+apply sepcon_derives. auto.
+apply sepcon_derives.
+{
+
+
+match goal with |- context [globvar2pred ?gv (?i, ?v)] =>
+  let i' := eval hnf in i in
+  let v' := eval hnf in v in 
+  change (globvar2pred gv (i,v)) with (globvar2pred gv (i',v'))
+ end.
+
+unfold globvar2pred; simpl.
+
+
+rewrite !sepcon_assoc.
+repeat apply sepcon_derives.
+admit.  (* stderrp *)
+apply derives
+f_equal.
+unfold globvar2pred.
+simpl gvar_volatile; cbv match.
+simpl gvar_init.
+simpl fst.
+
+entailer!!.
+cancel.
+
+ subst p; simpl. apply derives_refl. solve_SF_internal 
+    - 
+*)
