CertiGC/verif_is_ptr.v
@@ -1,10 +1,11 @@
-From CertiGraph.CertiGC Require Import env_graph_gc gc_spec.
-
-Ltac hif_tac H :=
-  match type of H with context [if ?a then _ else _] => destruct a eqn: ?H end.
+From CertiGraph.CertiGC Require Import env_graph_gc spec_gc.
 
 Lemma body_is_ptr: semax_body Vprog Gprog f_is_ptr is_ptr_spec.
 Proof.
-  start_function. forward_call x.
-  forward. red in H0. hif_tac H0. 2: inversion H1. destruct x; simpl in *; entailer!!.
+  start_function.
+  forward_call x.
+  forward.
+  red in H0.
+  destruct Archi.ptr64 eqn:H1; try solve [inversion H1].
+  destruct x; simpl in *; entailer!!.
 Qed.
